toolchain bump and bug fixing

Tests.lean
@@ -1,6 +1,8 @@
 import Lean4Less.Commands
 import patch.PatchTheoremsAx
 
+universe u v
+
 axiom P : Prop
 axiom Q : P → Prop
 axiom p : P
@@ -22,46 +24,45 @@ inductive K : Prop where
 --   (mk : motive 0 (K.mk a b)) {c : Nat}
 --   (t : K a b c) : motive c t
 
-axiom k : K
-axiom B : Bool → Type
-axiom hk : B (@K.rec (fun _ => Bool) true k)
+def k : K := (fun k => k) K.mk
+axiom BK : Bool → Type
+axiom hk : BK (@K.rec (fun _ => Bool) true k)
 
 -- succeeds because of K-like reduction
 -- (do not need constructor application to reduce)
-noncomputable def kLikeReduction : B true := hk
+noncomputable def kLikeReduction : BK true := hk
 
--- succeeds because of K-like reduction
--- (do not need constructor application to reduce)
--- theorem kLikeReduction' : B true := 
---    @L4L.castHEq (B (@K.rec (fun (x : K) => Bool) Bool.true k)) (B Bool.true)
---      (@L4L.appArgHEq Bool (fun (a : Bool) => Type) B (@K.rec (fun (x : K) => Bool) Bool.true k) Bool.true
---        (@L4L.appArgHEq K (fun (t : K) => (fun (x : K) => Bool) t) (@K.rec (fun (x : K) => Bool) Bool.true) k K.mk
---          (L4L.prfIrrel K k K.mk)))
---      hk
---
--- def ex' : T q Qq := 
---    @L4L.castHEq (T p Qp) (T q Qq)
---      (@L4L.appHEqABUV (Q p) (Q q) (fun (a : Q p) => Prop) (fun (a : Q q) => Prop)
---        (@L4L.appHEq P (fun (a : P) => Prop) Q Q p q (@HEq.refl (P → Prop) Q) (L4L.prfIrrelHEq P P (@HEq.refl Prop P) p q))
---        (fun (a : Q p) (a_1 : Q q) (a : @HEq (Q p) a (Q q) a_1) => @HEq.refl Type Prop) (T p) (T q) Qp Qq
---        (@L4L.appHEqUV P (fun (p : P) => Q _root_.p → Prop) (fun (p : P) => Q q → Prop)
---          (fun (p : P) =>
---            @L4L.forallHEqAB (Q _root_.p) (Q q) (fun (a : Q _root_.p) => Prop) (fun (a : Q q) => Prop)
---              (@L4L.appHEq P (fun (a : P) => Prop) Q Q _root_.p q (@HEq.refl (P → Prop) Q)
---                (L4L.prfIrrelHEq P P (@HEq.refl Prop P) _root_.p q))
---              fun (a : Q _root_.p) (a_1 : Q q) (a : @HEq (Q _root_.p) a (Q q) a_1) => @HEq.refl Type Prop)
---          T T p q (@HEq.refl ((p : P) → Q p → Prop) T) (L4L.prfIrrelHEq P P (@HEq.refl Prop P) p q))
---        (L4L.prfIrrelHEq (Q p) (Q q)
---          (@L4L.appHEq P (fun (a : P) => Prop) Q Q p q (@HEq.refl (P → Prop) Q)
---            (L4L.prfIrrelHEq P P (@HEq.refl Prop P) p q))
---          Qp Qq))
---      t
+axiom A : Type
+axiom a : A
+axiom h : Eq A A
+axiom h' : ∀ n : Nat, Q q
+theorem aux : (α β : Sort u) → (a : α) → (b : β) → HEq a b → (h : Eq α β) → Eq (cast h a) b :=
+  fun _ _ _ _ h₁ =>
+    h₁.rec (fun _ => rfl)
+axiom aux' : (α β : Sort u) → (a : α) → (b : β) → HEq a b → (h : Eq α β) → Eq (cast h a) b
 
--- example {α : Sort u} {a a' : α} (h : HEq a a') : Eq a a' :=
---   have : (α β : Sort u) → (a : α) → (b : β) → HEq a b → (h : Eq α β) → Eq (cast h a) b :=
---     fun A B a b h₁ =>
---       h₁.rec (fun _ => rfl)
---   this α α a a' h rfl
+def letFun' {α : Sort u} {β : α → Sort v} (v : α) (f : (x : α) → β x) : β v := f v
+
+theorem eq_of_heq' : ∀ {α : Sort u} {a a' : α}, @HEq α a α a' → @Eq α a a' :=
+   fun {α} {a a'} h =>
+     letFun' (fun α β a b h₁ =>
+       @HEq.rec α a (fun {B : Sort u} b _ => ∀ (h : @Eq (Sort u) α B), @Eq B (@cast α B h a) b)
+         (fun x => @rfl α (@cast α α x a)) β b h₁)
+     fun this => this α α a a' h (@rfl (Sort u) α)
+set_option pp.explicit true in
+
+#print eq_of_heq'
+
+noncomputable def ex : Q q :=
+  letFun' (α := Q p) Qq
+  fun this => this
+
+-- #print ex
+
+set_option pp.all true
+-- #check_off dif_pos
+#check_l4l ex
+-- #check_only Fin.mk_zero
 
 #check_l4l kLikeReduction
 -- axiom T : Type → Type
